{
 "cells": [
  {
   "cell_type": "markdown",
   "metadata": {},
   "source": [
    "# Exam 1"
   ]
  },
  {
   "cell_type": "markdown",
   "metadata": {},
   "source": [
    "1. Find the tangent line to $y = \\frac{1}{3}x^2$ at $x=1$\n",
    "\n",
    "$\\frac{d}{dx}\\left(\\frac{1}{3}x^2\\right) \\;=\\; \\frac{2}{3}x = f'(x)$\n",
    "\n",
    "$f'(1) = \\frac{2}{3}$\n",
    "\n",
    "$y_0 = f(1) = \\frac{1}{3}$\n",
    "\n",
    "$y-y_0 = f'(1)(x-x_0) \\quad \\to \\quad y-\\frac{1}{3} = \\frac{2}{3}(x-1)$\n",
    "\n",
    "**answer:** $\\quad\\quad y = \\frac{2}{3}x - \\frac{1}{3}$\n",
    "\n",
    "<br>"
   ]
  },
  {
   "cell_type": "markdown",
   "metadata": {},
   "source": [
    "---\n",
    "\n",
    "2. Find the derivative of the following functions:\n",
    "\n",
    "$\\text{a.}\\;\\;\\frac{x}{\\sqrt{1-x}}$\n",
    "\n",
    "$\\frac{d}{dx}\\left(\\frac{x}{\\sqrt{1-x}}\\right)$\n",
    "$\\;=\\; \\frac{\\frac{d}{dx}(x)\\sqrt{1-x}-\\frac{d}{dx}(\\sqrt{1-x})x}{(\\sqrt{1-x})^2} \\quad\\text{(Quotient Rule)}$\n",
    "\n",
    "$\\frac{d}{dx}(x) = 1$\n",
    "\n",
    "$\\frac{d}{dx}(\\sqrt{1-x})$\n",
    "\n",
    "$\\quad \\text{let } f=\\sqrt{u},\\;u=1-x\\quad\\text{(Chain Rule)}$\n",
    "\n",
    "$\\quad \\frac{d}{du}(\\sqrt{u})\\frac{d}{dx}(1-x)$\n",
    "\n",
    "$\\quad = \\frac{1}{2\\sqrt{u}}\\frac{d}{dx}(1-x)$\n",
    "$\\;=\\; \\frac{1}{2\\sqrt{1-x}}(-1) \\;=\\; \\frac{1}{2\\sqrt{1-x}}$\n",
    "\n",
    "$= \\frac{1 \\cdot \\sqrt{1-x} - \\left(-\\frac{1}{2\\sqrt{1-x}}\\right)x}{(\\sqrt{1-x})^2}$\n",
    "$\\;=\\; \\frac{\\sqrt{1-x}+\\frac{1}{2\\sqrt{1-x}}}{1-x} $\n",
    "$\\;=\\; \\frac{\\frac{2-x}{2\\sqrt{1-x}}}{1-x}$\n",
    "\n",
    "**answer:** $\\quad \\frac{2-x}{2\\sqrt{1-x}(1-x)}$\n",
    "\n",
    "<br>\n",
    "\n",
    "\n",
    "$\\text{b.}\\;\\;\\frac{\\cos(2x)}{x}$\n",
    "\n",
    "$\\frac{d}{dx}(\\frac{\\cos(2x)}{x}) = \\frac{\\frac{d}{dx}(\\cos(2x))x - \\frac{d}{dx}(x)\\cos(2x)}{x^2}\\quad \\text{(Quotient Rule)}$\n",
    "\n",
    "$\\frac{d}{dx}(x) = 1$\n",
    "\n",
    "$\\frac{d}{dx}(\\cos(2x))$\n",
    "\n",
    "$\\quad\\text{let }f=\\cos(u),\\;u=2x\\quad\\text{(Chain Rule)}$\n",
    "\n",
    "$\\quad\\frac{d}{du}(\\cos(u))\\frac{d}{dx}(2x)$\n",
    "$\\;=\\; -\\sin(u)\\cdot 2$\n",
    "$\\;=\\; -2\\sin(2x)$\n",
    "\n",
    "$= \\frac{(-2\\sin(2x))x - \\cos(2x)}{x^2}$\n",
    "\n",
    "**answer:** $\\quad \\frac{-2x\\sin(2x)-\\cos(2x)}{x^2}$\n",
    "\n",
    "<br>\n",
    "\n",
    "$\\text{c.}\\;\\;e^{2f(x)} = g(x)$\n",
    "\n",
    "**answer:** $\\frac{d}{dx}(g(x)) = 2\\frac{d}{dx}(f(x)) e^{2f(x)}$\n",
    "\n",
    "<br>\n",
    "\n",
    "$\\text{d.}\\;\\;\\ln(\\sin(x))$\n",
    "\n",
    "$\\frac{d}{dx}(\\ln(\\sin(x)))$\n",
    "\n",
    "$\\text{let } f=\\ln(u),\\;u=\\sin(x)\\quad\\text{(Chain Rule)}$\n",
    "\n",
    "$\\frac{d}{du}(\\ln(u))\\frac{d}{dx}(\\sin(x))$\n",
    "$\\;=\\; \\frac{1}{u}\\frac{d}{dx}(\\sin(x))$\n",
    "$\\;=\\; \\frac{1}{\\sin(x)}\\frac{d}{dx}(\\sin(x))$\n",
    "\n",
    "$\\frac{d}{dx}(sin(x)) = \\cos(x)$\n",
    "\n",
    "$= \\frac{1}{\\sin(x)}\\cos(x) \\;=\\; \\frac{\\cos(x)}{\\sin(x)} \\;=\\; \\cot(x)$\n",
    "\n",
    "**answer:** $\\quad \\cot(x)$\n",
    "\n",
    "<br>"
   ]
  },
  {
   "cell_type": "markdown",
   "metadata": {},
   "source": [
    "---\n",
    "\n",
    "3. Find $\\frac{dy}{dx}$ for the function $y$ defined implicitly by $y^4 + xy = 4 \\text{ at } x=3,\\;y=1$\n",
    "\n",
    "$\\frac{d}{dx}(y^4+xy) = \\frac{d}{dx}(4)$\n",
    "\n",
    "$\\frac{d}{dx}(y^4+xy) = \\frac{d}{dx}(y^4)+\\frac{d}{dx}(xy)$\n",
    "\n",
    "$\\frac{d}{dx}(y^4)$\n",
    "$\\;=\\; 4y^3\\frac{d}{dx}(y)$\n",
    "\n",
    "$\\frac{d}{dx}(xy)$\n",
    "$\\;=\\; \\frac{d}{dx}(x)y + \\frac{d}{dx}(y)x$\n",
    "$\\;=\\; 1y + x\\frac{d}{dx}(y)$\n",
    "\n",
    "<br>\n",
    "\n",
    "$4y^3\\frac{d}{dx}(y) + y + x\\frac{d}{dx}(y) = 0$\n",
    "\n",
    "$4y^3\\frac{d}{dx}(y) + x\\frac{d}{dx}(y) = -y$\n",
    "\n",
    "$\\frac{d}{dx}(y)(4y^3+x)) = -y$\n",
    "\n",
    "$\\frac{d}{dx}(y) = -\\frac{y}{4y^3+x}$\n",
    "\n",
    "<br>\n",
    "\n",
    "$\\frac{d}{dx}(y) \\;=\\; \\frac{-(1)}{4(1)^3 + (3)} \\;=\\; -\\frac{1}{7}$\n",
    "\n",
    "**answer:** $\\quad-\\frac{1}{7}$\n",
    "\n",
    "<br>"
   ]
  },
  {
   "cell_type": "markdown",
   "metadata": {},
   "source": [
    "---\n",
    "\n",
    "4. Let $fx=\n",
    "\\begin{cases}\n",
    "ax+b \\quad x\\lt 1 \\\\\n",
    "x^4+x+1 \\quad x\\ge 1 \n",
    "\\end{cases}$\n",
    "\n",
    "Find all $a$ and $b$ such that the function $f(x)$ is differentiable.\n",
    "\n",
    "\n",
    "$\\lim_{x \\to 1^-} (ax + b) \\;=\\; a+b$\n",
    "\n",
    "$\\lim_{x \\to 1^+} (x^4+x+1) \\;=\\; 3$\n",
    "\n",
    "Continuous at $x=1$ when $a+b=3$\n",
    "<br>\n",
    "\n",
    "$\\frac{d}{dx}(x^4+x+1) \\;=\\; 4x^3+1$\n",
    "\n",
    "$\\lim_{x \\to 1^-} (a) = a$\n",
    "\n",
    "$\\lim_{x \\to 1^+}(4x^3+1) = 5$\n",
    "\n",
    "$a + b = 3 \\quad\\to\\quad (5)+b=3$\n",
    "\n",
    "**answer:** $\\quad a=5,\\;b=-2$\n",
    "\n",
    "<br>"
   ]
  },
  {
   "cell_type": "markdown",
   "metadata": {},
   "source": [
    "---\n",
    "\n",
    "5. Derive the formula $\\frac{d}{dx}a^x = M(a)a^x$ directly from the definition of the derivative, and identify M(a) as a limit.\n",
    "\n",
    "$\\frac{d}{dx}(a^x) = \\lim_{b\\to 0}\\frac{a^{x+b}-a^x}{b}$\n",
    "$\\;=\\;\\lim_{b\\to 0}\\frac{a^xa^b-a^x}{b}$\n",
    "\n",
    "$=\\lim_{b\\to 0}\\frac{a^x(a^b-1)}{b}$\n",
    "$\\;=\\;a^x\\lim_{b\\to 0}\\frac{a^b-1}{b} \\equiv M(a)$"
   ]
  }
 ],
 "metadata": {
  "kernelspec": {
   "display_name": "Python 3.6.9 64-bit",
   "language": "python",
   "name": "python36964bit02ef2681bbc5400fadc04eb658c88111"
  },
  "language_info": {
   "codemirror_mode": {
    "name": "ipython",
    "version": 3
   },
   "file_extension": ".py",
   "mimetype": "text/x-python",
   "name": "python",
   "nbconvert_exporter": "python",
   "pygments_lexer": "ipython3",
   "version": "3.6.9"
  }
 },
 "nbformat": 4,
 "nbformat_minor": 4
}
