{
 "cells": [
  {
   "cell_type": "markdown",
   "metadata": {},
   "source": [
    "# Chapter 4 - Higher-Order Differential Equations"
   ]
  },
  {
   "cell_type": "markdown",
   "metadata": {},
   "source": [
    "## 4.1 - Preliminary Theory - Linear Equations"
   ]
  },
  {
   "cell_type": "markdown",
   "metadata": {},
   "source": [
    "**1.** Find a member of the given family of functions that is the solution of the initial value problem.\n",
    "\n",
    "- $y=c_1e^x+c_2e^{-x},\\quad (-\\infty,\\infty)$\n",
    "- $y''-y=0,\\quad y(0)=0,\\quad y'(0)=1$\n",
    "\n",
    "$(x,y)=(0,0)$\n",
    "\n",
    "$0 = c_1e^0+c_2e^0$\n",
    "$\\implies c_1+c_2=0$\n",
    "\n",
    "<br>\n",
    "\n",
    "$(x,y')=(0,1)$\n",
    "\n",
    "$y'=c_1e^x-c_2e^{-x}$\n",
    "\n",
    "$1=c_1e^0-c_2e^0\\implies c_1-c_2=1$\n",
    "\n",
    "<br>\n",
    "\n",
    "$c_1=\\frac{1}{2},\\quad c_2=-\\frac{1}{2}$\n",
    "\n",
    "$y=\\frac{1}{2}e^x-\\frac{1}{2}e^{-x}$"
   ]
  },
  {
   "cell_type": "markdown",
   "metadata": {},
   "source": [
    "<hr>\n",
    "\n",
    "**3.** Find a member of the given family of functions that is the solution of the initial value problem.\n",
    "\n",
    "- $y=c_1x+c_2x\\ln x,\\quad (0,\\infty)$\n",
    "- $x^2y''-xy'+y=0,\\quad y(1)=3,\\quad y'(1)=-1$\n",
    "\n",
    "$(x,y)=(1,3)$\n",
    "\n",
    "$3=c_1(1)+c_2(1)\\ln(1)$\n",
    "\n",
    "$3=c_1+c_2(0)\\implies c_1=3$\n",
    "\n",
    "<br>\n",
    "\n",
    "$y'=c_1+c_2\\ln(x)+c_2x\\frac{1}{x}$\n",
    "\n",
    "$y'=c_1+c_2(\\ln(x)+1)$\n",
    "\n",
    "$(x,y')=(1,-1)$\n",
    "\n",
    "$-1=c_1+c_2(\\ln(1)+1)$\n",
    "\n",
    "$-1=c_1+c_2(0+1)\\implies c_1+c_2=-1$\n",
    "\n",
    "<br>\n",
    "\n",
    "$c_1=3,\\quad c_2=-4$\n",
    "\n",
    "$y=3x-4x\\ln(x)$"
   ]
  },
  {
   "cell_type": "markdown",
   "metadata": {},
   "source": [
    "<hr>\n",
    "\n",
    "**7.** Given that $x(t)=c_1\\cos(wt)+c_2\\sin(wt)$ is the general solution of $x''+w^2x=0$ on the interval \n",
    "$(-\\infty,\\infty)$, show that a solution satisfying the initial conditions $x(0)=x_0,\\quad x'(0)=x_1$ is given by\n",
    "$x(t)=x_0\\cos(wt)+\\frac{x_1}{w}\\sin(wt)$\n",
    "\n",
    "$x(0)=x_0$\n",
    "\n",
    "$c_1\\cos w(0)+c_2\\sin w(0)=x_0$\n",
    "$\\implies c_1=x_0$\n",
    "\n",
    "<br>\n",
    "\n",
    "$x'(t)=-wc_1\\sin wt +wc_2\\cos wt$\n",
    "\n",
    "$x'(0)=x_1$\n",
    "\n",
    "$-wc_1\\sin w(0)+wc_2\\cos w(0)=x_1$\n",
    "$\\implies c_2=\\frac{x_1}{w}$\n",
    "\n",
    "<br>\n",
    "\n",
    "$x(t)=x_0\\cos wt+\\frac{x_1}{w}\\sin wt$"
   ]
  },
  {
   "cell_type": "markdown",
   "metadata": {},
   "source": [
    "<hr>\n",
    "\n",
    "**9.** Find interval centered about $x=0$ for which the given initial-value problem has a unique solution \n",
    "\n",
    "- $(x-2)y''+3y=x$\n",
    "- $y(0)=0,\\quad y'(0)=1$\n",
    "\n",
    "$a_2(x)\\frac{d^2y}{dx^2}+a_1(x)\\frac{dy}{dx}+a_0(x)=g(x)$\n",
    "\n",
    "$a_2(x)=x-2,\\quad a_1(x)=0,\\quad a_0(x)=3,\\quad g(x)=x$\n",
    "\n",
    "$(-\\infty, 2), (2,\\infty)\\quad a_2(2)=0 \\implies (-\\infty, 2)$"
   ]
  },
  {
   "cell_type": "markdown",
   "metadata": {},
   "source": [
    "<hr>\n",
    "\n",
    "**15.** Determine whether the given set of functions is linearly independent on the interval $(-\\infty,\\infty)$.\n",
    "\n",
    "- $f_1(x)=x$\n",
    "- $f_2(x)=x^2$\n",
    "- $f_3(x)=4x-3x^2$\n",
    "\n",
    "$W(f_1,f_2,f_3)=$\n",
    "$\\begin{vmatrix}f_1&f_2&f_3\\\\f'_1&f'_2&f'_3\\\\f''_1&f''_2&f''_3\\end{vmatrix}$\n",
    "$=\\begin{vmatrix}x&x^2&4x-3x^2\\\\1&2x&4-6x\\\\0&2&-6\\end{vmatrix}$\n",
    "\n",
    "$\\det(W(f_1,f_2,f_3))=$\n",
    "\n",
    "$=x\\cdot\\begin{vmatrix}2x&4-6x\\\\2&-6\\end{vmatrix}$\n",
    "$-x^2\\cdot\\begin{vmatrix}1&4-6x\\\\0&-6\\end{vmatrix}$\n",
    "$+(4x-3x^2)\\cdot\\begin{vmatrix}1&2x\\\\0&2\\end{vmatrix}$\n",
    "\n",
    "$=x\\left[(2x)(-6)-(4-6x)(2)\\right]-x^2\\left[(1)(-6)-(4-6x)(0)\\right]+(4x-3x^2)\\left[(1)(2)-(2x)(0)\\right]$\n",
    "\n",
    "$=x(-12x-8+12x)-x^2(-6)+(4x-3x^2)(2)$\n",
    "\n",
    "$=-8x^2+6x^2+8x^2-6x^2$\n",
    "\n",
    "$=0$\n",
    "\n",
    "The set is linearly dependent on the interval"
   ]
  },
  {
   "cell_type": "markdown",
   "metadata": {},
   "source": [
    "<hr>\n",
    "\n",
    "**23.** Verify that the given functions form a fundamental set of solutions of the differential equation on the indicated interval. Form the general solution.\n",
    "\n",
    "- $y''-y'-12y=0$\n",
    "- $e^{-3x},\\quad e^{4x},\\quad (-\\infty,\\infty)$\n",
    "\n",
    "$y=e^{-3x},\\quad y'=-3x^{-3x},\\quad y''=9e^{-3x}$\n",
    "\n",
    "$y''-y'-12y=0$\n",
    "\n",
    "$9e^{-3x}+3e^{-3x}-12e^{-3x}=0$\n",
    "\n",
    "$0=0$\n",
    "\n",
    "<br>\n",
    "\n",
    "$y=e^{4x},\\quad y'=4e^4x,\\quad y''=16e^{4x}$\n",
    "\n",
    "$y''-y'-12y=0$\n",
    "\n",
    "$16e^{4x}-4e^{4x}-12e^{4x}=0$\n",
    "\n",
    "$0=0$\n",
    "\n",
    "<br>\n",
    "\n",
    "$W(e^{-3x},e^{4x})=$\n",
    "$\\begin{vmatrix}e^{-3x}&e^{4x}\\\\-3e^{-3x}&4e^{4x}\\end{vmatrix}$\n",
    "$=e^{-3x}(4e^{4x})-e^{4x}(-3e^{-3x})$\n",
    "\n",
    "$=4e^x+3x^x\\implies 7e^x$\n",
    "\n",
    "$W(e^{-3x},e^{4x})=7e^x\\ne 0\\implies$ linearly independent\n",
    "\n",
    "$y=c_1e^{-3x}+c_2e^{4x}$"
   ]
  },
  {
   "cell_type": "markdown",
   "metadata": {},
   "source": [
    "<hr>\n",
    "\n",
    "**31.** Verify that the given two-parameter family of functions is the general solution of the nonhomogenous differential equation on the indicated interval.\n",
    "\n",
    "- $y''-7y'+10y=24e^x$\n",
    "- $y=c_1e^{2x}+c_2e^{5x}+6e^x,\\quad (-\\infty,\\infty)$\n",
    "\n",
    "$y_1=e^{2x},\\quad y_1'=2e^{2x},\\quad y_1''=4e^{2x}$\n",
    "\n",
    "$y''-7y'+10y=24e^x$\n",
    "\n",
    "$4e^{2x}-7(2e^{2x})+10(e^{2x})=0$\n",
    "$\\implies 0=0$\n",
    "\n",
    "<br>\n",
    "\n",
    "$y_2=e^{5x},\\quad y_2'=5e^{5x},\\quad y_2''=25e^{5x}$\n",
    "\n",
    "$25e^{5x}-7(5e^{5x})+10(e^{5x})=0$\n",
    "$\\implies 0=0$\n",
    "\n",
    "<br>\n",
    "\n",
    "$W(e^{2x},e^{5x})=$\n",
    "$\\begin{vmatrix}e^{2x}&e^{5x}\\\\2e^{2x}&5e^{5x}\\end{vmatrix}$\n",
    "$=(e^{2x})(5e^{5x})-(e^{5x})(2e^{2x})$\n",
    "\n",
    "$=5e^{7x}-2e^{7x}= 3e^{7x}\\implies$ linearly independent\n",
    "\n",
    "<br>\n",
    "\n",
    "$y_p=6e^x,\\quad y'_p=6e^x,\\quad y''_p=6e^x$\n",
    "\n",
    "$6e^x-7(6e^x)+10(6e^x)=24e^x$\n",
    "\n",
    "$66e^x-42e^x=24e^x$\n",
    "\n",
    "$24e^x=24e^x$\n",
    "\n",
    "So, $y_p$ satisfies the DE.\n",
    "\n",
    "<br>\n",
    "\n",
    "The general solution $y=c_1e^{2x}+c_2e^{5x}+6e^x$ is valid\n",
    "on the interval $(-\\infty,\\infty)$."
   ]
  },
  {
   "cell_type": "markdown",
   "metadata": {},
   "source": [
    "## 4.2 - Reduction of Order"
   ]
  },
  {
   "cell_type": "markdown",
   "metadata": {},
   "source": [
    "**1.** Use reduction of order or formula (5) to find a second solution $y_2(x)$ given a solution of the given differential equation $y_1(x)$.\n",
    "\n",
    "- $y''-4y'+4y=0$\n",
    "- $y_1=e^{2x}$\n",
    "\n",
    "$y''+p(x)y'+q(x)y=0$\n",
    "$\\implies p(x)=-4,\\quad q(x)=4$\n",
    "\n",
    "$y_1(x)=e^{2x}$\n",
    "\n",
    "$y_2(x)=y_1(x)\\int\\frac{e^{-\\int p(x)dx}}{(y_1)^2}dx$\n",
    "\n",
    "$=e^{2x}\\int\\frac{e^{-\\int -4dx}}{(e^{2x})^2}dx$\n",
    "\n",
    "$=e^{2x}\\int\\frac{e^4x}{e^4x}dx$\n",
    "\n",
    "$=e^{2x}x$"
   ]
  },
  {
   "cell_type": "markdown",
   "metadata": {},
   "source": [
    "<hr>\n",
    "\n",
    "**3.** Use reduction of order or formula (5) to find a second solution $y_2(x)$ given a solution of the given differential equation $y_1(x)$.\n",
    "\n",
    "- $y''+16y=0$\n",
    "- $y_1=\\cos(4x)$\n",
    "\n",
    "$y''+p(x)y'+q(x)y=0$\n",
    "$\\implies p(x)=0,\\quad q(x)=16$\n",
    "\n",
    "$y_1=\\cos(4x)$\n",
    "\n",
    "$y_2(x)=y_1(x)\\int\\frac{e^{-\\int p(x)dx}}{(y_1)^2}dx$\n",
    "\n",
    "$=\\cos(4x)\\int\\frac{e^{-\\int 0dx}}{(\\cos(4x))^2}dx$\n",
    "\n",
    "$=\\cos(4x)\\int\\frac{k}{\\cos^2(4x)}dx$\n",
    "\n",
    "$=\\cos(4x)\\int k\\sec^2 4xdx$\n",
    "\n",
    "$=\\cos(4x)(k)\\cdot\\frac{1}{4}\\tan4x$\n",
    "\n",
    "$=\\frac{k}{4}\\sin4x$\n",
    "\n",
    "$=c_2\\sin 4x = \\sin 4x$"
   ]
  },
  {
   "cell_type": "markdown",
   "metadata": {},
   "source": [
    "## 4.3 - Homogenous Linear Equations with Constant Coefficients"
   ]
  },
  {
   "cell_type": "markdown",
   "metadata": {},
   "source": [
    "**1.** Find the general solution of the given second-order differential equation. \n",
    "$\\quad 4y''+y'=0$\n",
    "\n",
    "$y=e^{mx},\\quad y'=me^{mx},\\quad y''=m^2e^{mx}$\n",
    "\n",
    "$4m^2e^{mx}+me^{mx}=0$\n",
    "\n",
    "$e^{mx}(4m^2+m)=0$\n",
    "\n",
    "$4m^2+m=0$\n",
    "\n",
    "$m(4m+1)=0\\implies m_1=0,\\;m_2=-\\frac{1}{4}$\n",
    "\n",
    "$y=c_1e^{m_1x}+c_2e^{m_2x}$\n",
    "\n",
    "$=c_1e^0+c_2e^{-\\frac{1}{4}x}$\n",
    "\n",
    "$=c_1+c_2e^{-\\frac{1}{4}x}$"
   ]
  },
  {
   "cell_type": "markdown",
   "metadata": {},
   "source": [
    "<hr>\n",
    "\n",
    "**3.** Find the general solution of the given second-order differential equation. \n",
    "$\\quad y''-y'-6y=0$\n",
    "\n",
    "$y=e^{mx},\\quad y'=me^{mx},\\quad y''=m^2e^{mx}$\n",
    "\n",
    "$m^2e^{mx}-me^{mx}-6e^{mx}=0$\n",
    "\n",
    "$e^{mx}(m^2-m-6)=0$\n",
    "\n",
    "$m^2-m-6=0$\n",
    "\n",
    "$(m-3)(m+2)=0\\implies m_1=3,\\; m_2=-2$\n",
    "\n",
    "$y=c_1e^{m_1x}+c_2e^{m_2x}$\n",
    "\n",
    "$=c_1e^{3x}+c_2e^{-2x}$"
   ]
  },
  {
   "cell_type": "markdown",
   "metadata": {},
   "source": [
    "<hr>\n",
    "\n",
    "**29.** Solve the given initial-value problem.\n",
    "\n",
    "- $y''+16y=0$\n",
    "- $y(0)=2,\\quad y'(0)=-2$\n",
    "\n",
    "$y=e^{mx},\\quad y'=me^{mx},\\quad y''=m^2e^{mx}$\n",
    "\n",
    "$m^2e^{mx}+16e^{mx}=0$\n",
    "\n",
    "$e^{mx}(m^2+16)=0$\n",
    "\n",
    "$m^2+16=0 \\implies m_1=m_2=\\sqrt{-16}=\\pm 4i$\n",
    "\n",
    "<br>\n",
    "\n",
    "$y=c_1e^{4ix}+c_2e^{-4ix}$\n",
    "\n",
    "$=c_1e^0(\\cos(4x)+\\sin(4x))+c_2e^0(\\cos(4x)-\\sin(4x))$\n",
    "\n",
    "$=k_1\\cos(4x)+k_2\\sin(4x)$, where $k_1=c_1+c_2$ and $k_2=c_1-c_2$\n",
    "\n",
    "<br>\n",
    "\n",
    "$(x,y)=(0,2)$\n",
    "\n",
    "$2=k_1\\cos(0)+k_2\\sin(0)\\implies k_1=2$\n",
    "\n",
    "$y'=-4k_1\\sin(4x)+4k_2\\cos(4x)$\n",
    "\n",
    "<br>\n",
    "\n",
    "$(x,y')=(0,-2)$\n",
    "\n",
    "$-2=-4k_1\\sin(0)+4k_2\\cos(0)$\n",
    "\n",
    "$4k_2=-2\\implies k_2=-\\frac{1}{2}$\n",
    "\n",
    "<br>\n",
    "\n",
    "$y=2\\cos(4x)-\\frac{1}{2}\\sin(4x)$"
   ]
  },
  {
   "cell_type": "markdown",
   "metadata": {},
   "source": [
    "## 4.5 - Undetermined Coefficients - Annihilator Approach"
   ]
  },
  {
   "cell_type": "markdown",
   "metadata": {},
   "source": [
    "**1.** Write the given differential equation in the form $L(y)=g(x)$, where $L$ is a linear differential operator with constant coefficients. If possible, factor $L$. $\\quad 9y''-4y=\\sin(x)$\n",
    "\n",
    "$9D^2y-4y=\\sin x$\n",
    "\n",
    "$(9D^2-4)y=\\sin x$\n",
    "\n",
    "$(3D-2)(3D+2)y=\\sin x$"
   ]
  },
  {
   "cell_type": "markdown",
   "metadata": {},
   "source": [
    "<hr>\n",
    "\n",
    "**3.** Write the given differential equation in the form $L(y)=g(x)$, where $L$ is a linear differential operator with constant coefficients. If possible, factor $L$. $\\quad y''-4y'-12y=x-6$\n",
    "\n",
    "\n",
    "$D^2y-4Dy-12y=x-6$\n",
    "\n",
    "$(D^2-4D-12)y=x-6$\n",
    "\n",
    "$(D+2)(D-6)y=x-6$"
   ]
  },
  {
   "cell_type": "markdown",
   "metadata": {},
   "source": [
    "<hr>\n",
    "\n",
    "**11.** Verify that the given differential operator annihilates the indicated functions.\n",
    "\n",
    "- $D^4$\n",
    "- $y=10x^3-2x$\n",
    "\n",
    "$D^4y=D^4(10x^3-2x)$\n",
    "\n",
    "$D^4y=D^3(30x^2-2)$\n",
    "\n",
    "$D^4y=D^2(60x)$\n",
    "\n",
    "$D^4y=D(60)$\n",
    "\n",
    "$D^4y=0$"
   ]
  },
  {
   "cell_type": "markdown",
   "metadata": {},
   "source": [
    "<hr>\n",
    "\n",
    "**15.** Find a linear differential operator that annihilates the given function. $\\quad 1+6x-2x^3$\n",
    "\n",
    "$1 \\to D^1$\n",
    "\n",
    "$6x \\to D^2$\n",
    "\n",
    "$-2x^3 \\to D^4$\n",
    "\n",
    "$D^4(1+6x-2x^3)=0$"
   ]
  },
  {
   "cell_type": "markdown",
   "metadata": {},
   "source": [
    "<hr>\n",
    "\n",
    "**17.** Find a linear differential operator that annihilates the given function. $\\quad 1+7e^{2x}$\n",
    "\n",
    "$1 \\to D^1$\n",
    "\n",
    "$7e^{2x} \\to (D-2)$\n",
    "\n",
    "$D(D-2)(1+7e^{2x})=0$"
   ]
  },
  {
   "cell_type": "markdown",
   "metadata": {},
   "source": [
    "<hr>\n",
    "\n",
    "**35.** Solve the given differential equation by undetermined coefficients. $\\quad y''-9y=54$\n",
    "\n",
    "$y''-9y=0$\n",
    "\n",
    "$y=e^{mx},\\quad y'=me^{mx},\\quad y''=m^2e^{mx}$\n",
    "\n",
    "$m^2e^{mx}-9e^{mx}=0$\n",
    "\n",
    "$e^{mx}(m^2-9)=0$\n",
    "\n",
    "$m^2-9=0$\n",
    "\n",
    "$(m-3)(m+3)=0 \\implies m_1=3,\\;m_2=-3$\n",
    "\n",
    "homogenous solution: $\\quad y=c_1e^{3x}+c_2e^{-3x}$\n",
    "\n",
    "<br>\n",
    "\n",
    "$D^2y-9y=54$\n",
    "\n",
    "$(D^2-9)y=54$\n",
    "\n",
    "$D(D^2-9)y=D(54)$\n",
    "\n",
    "$D(D^2-9)y=0$\n",
    "\n",
    "<br>\n",
    "\n",
    "$m(m^2-9)=0$\n",
    "\n",
    "$(m-3)(m+3)m=0\\implies m_1=3,m_2=-3,m_3=0$\n",
    "\n",
    "$y=k_1e^{3x}+k_2e^{-3x}+k_3e^0$\n",
    "\n",
    "$y_p=k_3,\\quad y'_p=0,\\quad y''_p=0$\n",
    "\n",
    "Let $y_p=A \\implies \\quad 0-9A=54 \\implies A=-6$\n",
    "\n",
    "$y_p=-6$\n",
    "\n",
    "$y=k_1e^{3x}+k_2e^{-3x}-6$"
   ]
  },
  {
   "cell_type": "markdown",
   "metadata": {},
   "source": [
    "## 4.6 - Variation of Parameters"
   ]
  },
  {
   "cell_type": "markdown",
   "metadata": {},
   "source": [
    "**1.** Solve the differential equation by variation of parameters. $\\quad y''+y=\\sec(x)$\n",
    "\n",
    "$y''+p(x)y'+q(x)y=f(x)$\n",
    "\n",
    "$y=e^{mx},\\quad y'=me^{mx},\\quad y''=m^2e^{mx}$\n",
    "\n",
    "$m^2e^{mx}+e^{mx}=0$\n",
    "\n",
    "$e^{mx}(m^2+1)=0$\n",
    "\n",
    "$m^2+1=0\\implies m_1=m_2=\\pm i$\n",
    "\n",
    "$y_h=c_1y_1+c_2y_2$\n",
    "\n",
    "$=c_1\\cos x+c_2\\sin x$\n",
    "\n",
    "<br>\n",
    "\n",
    "$W(y_1,y_2)=$\n",
    "$\\begin{vmatrix}\\cos x&\\sin x\\\\-\\sin x&\\cos x\\end{vmatrix}$\n",
    "$=\\cos^2x-(-\\sin^2x)$\n",
    "$=1$\n",
    "\n",
    "$W_1=\\begin{vmatrix}0&y_2\\\\f(x)&y'_2\\end{vmatrix}$\n",
    "$=\\begin{vmatrix}0&\\sin x\\\\\\sec x&\\cos x\\end{vmatrix}$\n",
    "$=0-(\\sin x)(\\sec x)$\n",
    "\n",
    "$=-\\tan x$\n",
    "\n",
    "$W_2=\\begin{vmatrix}y_1&0\\\\y'_1&f(x)\\end{vmatrix}$\n",
    "$=\\begin{vmatrix}\\cos x&0\\\\-\\sin x&\\sec x\\end{vmatrix}$\n",
    "$=(\\cos x)(\\sec x)-0$\n",
    "$=1$\n",
    "\n",
    "<br>\n",
    "\n",
    "$u'_1=\\frac{W_1}{W(y_1,y_2)}$\n",
    "$=\\frac{-\\tan x}{1}=-\\tan x$\n",
    "\n",
    "$u'_2=\\frac{W_2}{W(y_1,y_2)}$\n",
    "$=\\frac{1}{1}=1$\n",
    "\n",
    "$u_1=\\int u'_1dx$\n",
    "$=\\int -\\tan x dx$\n",
    "$=\\int -\\frac{\\sin x}{\\cos x}dx$\n",
    "$=\\ln(\\cos x)$\n",
    "\n",
    "$u_2=\\int u'_2dx$\n",
    "$=\\int 1dx = x$\n",
    "\n",
    "<br>\n",
    "\n",
    "$y_p=u_1y_1+u_2y_2$\n",
    "$=\\ln(\\cos x)(\\cos x)+x\\sin x$\n",
    "\n",
    "$y=y_h+y_p$\n",
    "\n",
    "$y = c_1\\cos x+c_2\\sin x+\\cos x\\ln(\\cos x)+x\\sin x$"
   ]
  },
  {
   "cell_type": "markdown",
   "metadata": {},
   "source": [
    "## 4.7 - Cauchy-Euler Equation"
   ]
  },
  {
   "cell_type": "markdown",
   "metadata": {},
   "source": [
    "**1.** Solve the given differential equation. $\\quad x^2y''-2y=0$\n",
    "\n",
    "$x^2\\frac{d^2y}{dx^2}-2y=0$\n",
    "\n",
    "$y=x^m$\n",
    "\n",
    "$\\frac{dy}{dx}=mx^{m-1}$\n",
    "\n",
    "$\\frac{d^2y}{dx^2}=m(m-1)x^{m-2}$\n",
    "\n",
    "<br>\n",
    "\n",
    "$x^2\\frac{d^2y}{dx^2}-2y=0$\n",
    "\n",
    "$x^2m(m-1)x^{m-2}=0$\n",
    "\n",
    "$x^m(m(m-1)-2)=0$\n",
    "\n",
    "$x^m(m^2-m-2)=0$\n",
    "\n",
    "$m^2-m-2=0\\implies (m+1)(m-2)=0$\n",
    "\n",
    "$m_1=-1,\\quad m_2=2$\n",
    "\n",
    "<br>\n",
    "\n",
    "$y=c_1x^{m_1}+c_2x^{m_2}$\n",
    "\n",
    "$y=c_1x^{-1}+c_2x^2$"
   ]
  },
  {
   "cell_type": "markdown",
   "metadata": {},
   "source": [
    "<hr>\n",
    "\n",
    "**3.** Solve the given differential equation. $\\quad xy''+y'=0$\n",
    "\n",
    "$x\\frac{d^2y}{dx^2}+\\frac{dy}{dx}=0$\n",
    "\n",
    "$x^2\\frac{d^2y}{dx^2}+x\\frac{dy}{dx}=0(x)$\n",
    "\n",
    "$y=x^m,\\quad \\frac{dy}{dx}=mx^{m-1},\\quad\\frac{d^2y}{dx^2}=m(m-1)x^{m-2}$\n",
    "\n",
    "<br>\n",
    "\n",
    "$x^2\\frac{d^2y}{dx^2}+x\\frac{dy}{dx}=0$\n",
    "\n",
    "$x^2m(m-1)x^{m-2}+xmx^{m-1}=0$\n",
    "\n",
    "$x^m(m(m-1)+m)=0$\n",
    "\n",
    "$x^m(m^2)=0 \\implies m_1=m_2=0$\n",
    "\n",
    "<br>\n",
    "\n",
    "$y=c_1+c_2\\ln(x)$"
   ]
  }
 ],
 "metadata": {
  "kernelspec": {
   "display_name": "Python 3",
   "language": "python",
   "name": "python3"
  },
  "language_info": {
   "codemirror_mode": {
    "name": "ipython",
    "version": 3
   },
   "file_extension": ".py",
   "mimetype": "text/x-python",
   "name": "python",
   "nbconvert_exporter": "python",
   "pygments_lexer": "ipython3",
   "version": "3.6.5"
  }
 },
 "nbformat": 4,
 "nbformat_minor": 4
}
